\section{Example: The Weyl Algebra}


\begin{fluff}
  To motivate the upcoming theorem of Poincaré--Birkhoff--Witt and its proof we consider first another example.
\end{fluff}


\begin{definition}
  The \defemph{Weyl algebra} is the~\algebra{$\kf$}~$\kf\gen{X, Y} / \ideal{YX - XY - 1}$.%
  \footnote{The algebra~$A$ is isomorphic to the subalgebra of~$\End_{\kf}(\kf[t])$ generated by the endomorphisms~$x$ and~$y$ that are given by~$x(p(t)) = t p(t)$ and~$y(p(t)) = p'(t)$.
  These endomorphisms satsify the relations~$yx - xy - \id = 0$ by the product rule.}
\end{definition}


\begin{fluff}
  \label{filtration on the weyl algebra}
  Let~$A = \kf\gen{X,Y} / \ideal{YX - XY - 1}$ be the Weyl algebra.
  We denote the residue classes of~$X$ and~$Y$ in~$A$ by~$x$ and~$y$.
  Then~$yx = xy + 1$, which one may think about as a rewriting rule for words in~$x$ and~$y$.
  It follows by induction that
  \[
    y x^n
    =
    x^n y + n x^{n-1}
  \]
  for all~$n \geq 0$ and thus
  \[
    y p(x)
    =
    p(x) y + p'(x)
  \]
  for every polynomial~$p$.
  
  The free~{\algebra{$\kf$}}~$T \defined \kf\gen{X, Y}$ carries a unique grading with~$X$ and~$Y$ in degree~$1$.
  The resulting filtration of~$T$ is given by
  \[
    T_{(p)}
    =
    \gen{
      Z_1 \dotsm Z_q
    \suchthat
      0 \leq q \leq p,
      Z_q \in \{X, Y\}
    }_{\kf}
    =
    \gen{
      \text{words in~$X$,~$Y$ of length~$\leq p$}
    }_{\kf}
  \]
  The Weyl~algebra~$A$ inherits a filtration given by
  \begin{align*}
    A_{(p)}
    =
    \gen{
      z_1 \dotsm z_q
    \suchthat
      1 \leq q \leq p,
      z_q \in \{x, y\}
    }_{\kf}
    =
    \gen{
      \text{words in~$x$,~$y$ of length~$\leq p$}
    }_{\kf}
  \end{align*}
  
  We now observe that the two generators~$x$ and~$y$ of~$A$ commute up to smaller degree, i.e.\ the two products~$xy$ and~$yx$ are equal up to smaller degree.
  The associated elements~$\fclass{x}_1$ and~$\fclass{y}_1$ in~$\gr(A)$ do therefore actually commute, because
  \[
    \fclass{x}_1 \fclass{y}_1
    =
    \fclass{xy}_2
    =
    \fclass{yx - 1}_2
    =
    \fclass{ yx }2
    =
    \fclass{y}_1 \fclass{x}_1 \,.
  \]
  We will in the following show that~$\gr(A) \cong \kf[t,u]$ with the elements~$\fclass{x}_1$ and~$\fclass{y}_1$ corresponding to the commutative variables~$t$ and~$u$.
\end{fluff}


\begin{lemma}
  \label{subspace spanned by monomials}
  The linear subspace~$A_{(p)}$ of~$A$ is spanned by the monomial~$x^n y^m$ with~$n + m \leq p$, for every~$p \geq 0$.
\end{lemma}
  

\begin{proof}
  We show the statement by induction over~$p$.
  It holds for~$p = 0$ because
  \[
    A_{(0)}
    =
    \kf
    =
    \gen{1}_{\kf}
    =
    \gen{x^0 y^0}_{\kf} \,.
  \]
  Suppose now that the \lcnamecref{subspace spanned by monomials} holds for some~$p \geq 0$.
  We have
  \[
    T_{(p+1)}
    =
    x T_{(p)} \oplus y T_{(p)}
  \]
  and therefore
  \[
    A_{(p+1)}
    =
    x A_{(p)} + y A_{(p)} \,.
  \]
  We find by the induction hypothesis that the summand~$x A_{(p)}$ is spanned by all those monomials~$x^{n+1} y^m$ with~$n+m \leq p$ and that the summand~$y A_{(p)}$ is spanned by all those monomials~$y x^n y^m$ with~$n + m \leq p$.
  We have for these generators of~$y A_{(p)}$ that
  \[
    y x^n y^m
    =
    (x^n y + n x^{n-1}) y^m
    =
    x^n y^{m+1} + n x^{n-1} y^m \,.
  \]
  This shows that~$A_{(p+1)}$ is spanned by all those monomials~$x^n y^m$ with~$n+m \leq p+1$.
\end{proof}
 
\begin{fluff}
  It follows from \cref{subspace spanned by monomials} for every natural number~$p$ that the homogeneous component~$\gr[p](A)$ of~$\gr(A)$ is spanned by all those residue classes~$\fclass{ x^n y^m }_p$ with~$n + m = p$.
  It further follows that the algebra~$\gr(A)$ is spanned by the monomials~$\fclass{ x^n y^m }_p$ with~$p \geq 0$ and~$p = n + m$ as a vector space.

  We will now see that the multiplication of these vector space generators works in the naive way.
\end{fluff}
  
\begin{lemma}
  \label{generators commute for weyl}
  It holds for all~$p, q \geq 0$ and~$n, m, k, l \geq 0$ with~$p = n+m$ and~$q = k+l$ that
  \[
    \fclass{ x^n y^m }_p \cdot \fclass{ x^k y^l }_q
    =
    \fclass{ x^{n+k} y^{m+l} }_{p+q} \,.
  \]
\end{lemma}
  
\begin{proof}
  For the case~$p = 0$ we find that~$n = m = 0$ and hence
  \[
    \fclass{ x^0 y^0 }_0 \cdot \fclass{ x^k y^l }_q
    =
    \fclass{ 1 }_0 \cdot \fclass{ x^k y^l }_q
    =
    \fclass{ x^k y^l }_q
  \]
  For~$p = 1$ we have the two cases~$n = 1$,~$m = 0$ and~$n = 0$,~$m = 1$ to consider.
  We find in the first case that
  \[
    \fclass{ x^1 y^0 }_1 \cdot \fclass{ x^k y^l}_q
    =
    \fclass{x}_1 \cdot \fclass{ x^k y^l }_q
    =
    \fclass{x \cdot x^k y^l}_{q+1}
    =
    \fclass{ x^{k+1} y^l }_{q+1} \,.
  \]
  In the second case we find that
  \begin{align*}
    \fclass{ x^0 y^1 }_1 \cdot \fclass{ x^k y^l }_q
    &=
    \fclass{y}_1 \cdot \fclass{ x^k y^l }_q
    \\
    &=
    \fclass{ y x^k y^l }_{q+1}
    \\
    &=
    \fclass{ (x^k y + k x^{k-1}) y^l }_{q+1}
    \\
    &=
    \fclass{ x^k y^{l+1} + k x^{k-1} y^l }_{q+1}
    \\
    &=
    \fclass{ x^k y^{l+1} }_{q+1} + k \fclass{ x^{k-1} y^l] }{q+1}
    \\
    &=
    \fclass{ x^k y^{l+1} }_{q+1} \,,
  \end{align*}
  where we used that~$x y^k = y^k x + k y^{k-1}$ and that~$\fclass{ z }_{q+1} = 0$ for all~$z \in A_{(q)}$.
  It follows for the general case that
  \begin{align*}
    {}&
    \fclass{ x^n y^m }_p \cdot \fclass{ x^k y^l }_q
    \\
    ={}&
    \underbrace{ \fclass{x}_1 \dotsm \fclass{x}_1 }_{n}
    \underbrace{ \fclass{y}_1 \dotsm \fclass{y}_1 }_{m}
    \cdot
    \fclass{ x^k y^l }_q
    \\
    ={}&
    \underbrace{ \fclass{x}_1 \dotsm \fclass{x}_1 }_{n}
    \underbrace{ \fclass{y}_1 \dotsm \fclass{y}_1 }_{m-1}
    \cdot
    \fclass{ x^{1+k}  y^l }_{1+q}
    \\
    ={}&
    \dotsb
    \\
    ={}&
    \fclass{ x^{n+k} y^{m+l} }_{p+q} \,,
  \end{align*}
  as claimed.
\end{proof}


\begin{fluff}
  To show the desired isomorphism~$\gr(A) \cong \kf[t,u]$ we are still missing one key ingredient, namely the linear independence of the monomials~$[x_n y^m]_p$ with~$p \geq 0$,~$n, m \geq 0$,~$p = n+m$.
  This will follow from the next result.
\end{fluff}

  
\begin{lemma}
  \label{linear independence of monomials}
  The monomials~$x^n y^m$ with~$n, m \geq 0$ in~$A$ are linearly independent.
\end{lemma}


\begin{fluff}
  To prove \cref{linear independence of monomials} we will use a general trick from representation theory, which we will now explain.
\end{fluff}


\begin{construction}
  \label{representation theory trick to construct a basis}
  Let~$A$ be a~\algebra{$\kf$} and let~$(b_j)_{j \in J}$ be a vector space generating set of~$A$, which we would like to show to be a basis of~$A$.

  Suppose that we are somehow given an~{\module{$A$}}~$M$ together with an element~$m_0$ of~$M$ such that the family~$(b_j m_0)_{j \in J}$ is linearly dependent in~$M$.
  It then follows that the original family~$(b_j)_{j \in J}$ is also linearly independent.
  Indeed, if we have a linear combination
  \[
    \sum_{j \in J} \lambda_j b_j = 0
  \]
  then by acting upon the element~$m_0$ it follows that
  \[
    \sum_{j \in J} \lambda_j b_j m_0 = 0
  \]
  and thus~$\lambda_j = 0$ for all~$j \in J$.

  We therefore would like to construct such an~\module{$A$}~$M$.
  We make for this construction a basic observation:
  if~$(b_j)_{j \in J}$ really turns out to be a basis of~$A$, then we could -- a posteriori -- have choosen~$M = A$ and~$m_0 = 1$.
  In other words, we could have chosen~$M$ as a vector space with a basis indexed by~$J$, and have choosen the action of~$A$ on these basis elements \enquote{in the same way} as the action of~$A$ on the basis elements~$b_j$ of~$A$.

  To construct the desired module~$M$ we therefore let~$M$ be the free vector space with basis~$(B_j)_{j \in J}$.
  We want the algebra~$A$ to act on the vector space~$M$ in the same way as~$A$ acts on itself.
  How this action can be formally constructed depends on the given algebra~$A$ and family~$(b_j)_{j \in J}$.
  One possible way is as follows.

  Suppose that the algebra~$A$ is given by a family of algebra generators~$(x_i)_{i \in I}$ together with certain relations between these generators.
  The action of~$A$ on itself can be encoded as linear combination~$x_i b_j = \sum_{k \in J} c_{ij}^k b_k$ with~$i \in I$,~$j \in J$.
  We then want to define an action of~$A$ on the vector space~$M$ such that~$x_i B_j = \sum_{k \in J} c_{ij}^k B_k$ for all~$i \in I$,~$j \in J$.
  This can be done in two steps.
  \begin{enumerate}
    \item
      We first define a~\module{$\kf\gen{X_i \suchthat i \in I}$} structure on~$M$ via~$X_i \cdot B_j = \sum_{k \in I} c_{ij}^k B_k$.
      We can do this because a~\module{$\kf\gen{X_i \suchthat i \in I}$} structure on~$M$ is the same a homomorphism of algebras from~$\kf\gen{X_i \suchthat i \in I}$ to~$\End_{\kf}(M)$, which can be constructed by using the universal property of the free algebra~$\kf\gen{X_i \suchthat i \in I}$.
    \item
      We then check that this action descends to an~\module{$A$} structure on~$M$ by checking that it is compatible with the given relations between the algebra generators~$x_i$.
  \end{enumerate} 
  Suppose now that~$1 = b_k$ for some index~$k$.
  We then set~$m_0 \defined B_k$.
  Then~$b_j \act m_0 = B_j$ for all~$j \in J$, and these elements are linearly independent in~$M$.
\end{construction}

\begin{proof}[Proof of  \cref{linear independence of monomials}]
  \label{linear independence for weyl algebra}
  Let~$M$ be the free vector space with basis~$T^n U^m$ where~$n, m \geq 0$.
  We have
  \begin{align*}
    x \cdot x^n y^m
    &=
    x^{n+1} y^m \,,
    \\
    y \cdot x^n y^m
    &=
    x^n y^{m+1} + n x^{n-1} y^m
  \end{align*}
  for all~$n, m \geq 0$.
  We therefore define a~{\module{$\kf\gen{X,Y}$}} structure on~$M$ by
  \begin{align*}
    X \cdot T^n U^m
    &=
    T^{n+1} U^m \,,
    \\
    Y \cdot T^n U^m
    &=
    T^n U^{m+1} + n T^{n-1} U^m
  \end{align*}
  for all~$m, n \geq 0$.
  We have
  \begin{gather*}
    YX \cdot T^n U^m
    =
    Y \cdot T^{n+1} U^m
    =
    T^{n+1} U^{m+1} + (n+1) T^n U^m
  \shortintertext{and}
    XY \cdot T^n U^m
    =
    X \cdot ( T^n U^{m+1} + n T^{n-1} U^m )
    =
    T^{n+1} U^{m+1} + n T^n U^m
  \end{gather*}
  for all~$n, m \geq 0$ and thus
  \[
    (YX - XY - 1) \cdot T^n U^m
    =
    0
  \]
  for all~$n, m \geq 0$.
  The~\module{$\kf\gen{X,Y}$} structure on~$M$ therefore descends to an~\module{$A$} on~$M$.
  We have
  \[
    y \cdot T^0 U^m
    =
    Y \cdot T^0 U^m
    =
    T^0 U^{m+1}
  \]
  for all~$m \geq 0$, and therefore inductively
  \[
    y^k \cdot T^0 U^m
    =
    T^0 U^{m+k}
  \]
  for all~$k, m \geq 0$.
  It further follows that
  \[
    x^n y^m \cdot T^0 U^0
    =
    x^n \cdot T^0 U^m
    =
    T^n U^m
  \]
  for all~$n, m \geq 0$.

  It now follows from the linear independence of the basis elements~$T^n U^m$ of~$M$ that the elements~$x^n y^m$ of~$A$ are also linearly independent.
\end{proof}


\begin{fluff}
  We can summarize our findings as follows.
\end{fluff}


\begin{proposition}
  \label{results about the weyl algerba}
  Let~$A = \kf\gen{X,Y} / \ideal{YX - XY - 1}$ be the Weyl algebra.
  Let~$x$ be the residue class of~$X$ in~$A$ and let~$y$ be the residue class of~$Y$ in~$A$.
  \begin{enumerate}
    \item
      The algebra~$A$ admits a filtration given by
      \[
        A_{(p)}
        =
        \gen{
          z_1 \dotsm z_q
          \suchthat
          q \leq p,
          z_i \in \{ x, y \}
        }_{\kf}
        =
        \gen{
          \text{words in~$x$,~$y$ of length~$\leq p$}
        }_{\kf} \,.
      \]
    \item
      \label{basis for filtration of weyl algebra}
      The linear subspace~$A_{(p)}$ of~$A$ has the monomials~$x^n y^m$ with~$n, m \geq 0$,~$n + m \leq p$ as a basis, for all~$p \geq 0$.
    \item
      The algebra~$A$ has the monomials~$x^n y^m$ with~$n, m \geq 0$ as a basis.
    \item
      \label{homogeneous basis for associated graded of weyl algebra}
      The homogeneous component~$\gr[p](A)$ has the monomials~$\fclass{ x^n y^m }_p$ with~$n, m \geq 0$,~$p = n+m$ as a basis, for all~$p \geq 0$.
    \item
      \label{basis for associated graded of weyl algebra}
      The algebra~$\gr(A)$ has the monomials~$\fclass{ x^n y^m }_p$ with~$n, m \geq 0$,~$p = n+m$ as a basis.
    \item
      \label{multiplication on basis of associated graded of weyl algebra}
      The multiplicaiton of~$\gr(A)$ is given by
      \[
        \fclass{ x^n y^m }_p \cdot \fclass{ x^k y^l }_q
        =
        \fclass{ x^{n+k} y^{m+l} }_{p+q}
      \]
      for all~$n, m, k, l \geq 0$,~$p = n + m$,~$q = k + l$.
    \item
      The algebra~$\gr(A)$ is isomorphic to the polynomial algebra~$\kf[t,u]$ as graded algebra where~$x$ corresponds to~$t$ and~$y$ corresponds to~$u$.
  \end{enumerate}
\end{proposition}


\begin{proof}
  \leavevmode
  \begin{enumerate}
    \item
      This follows from \cref{filtration on the weyl algebra}.
    \item
      This follows from \cref{subspace spanned by monomials} and \cref{linear independence of monomials}.
    \item
      This follows from part~\ref{basis for filtration of weyl algebra}.
    \item
      This follows from part~\ref{basis for filtration of weyl algebra}.
    \item
      This follows from the previous part.
    \item
      This is \cref{generators commute for weyl}. 
    \item
      It follows from part~\ref{basis for associated graded of weyl algebra} that there exists an isomorphism of vector spaces between~$\gr(A)$ and~$\kf[t,u]$ such that~$\fclass{ x^n y^m }_p$ corresponds to~$t^n u^m$ for all~$n, m \geq 0$.
      This is an isomorphism of algebras by part~\ref{multiplication on basis of associated graded of weyl algebra}, and finally an isomorphism of graded algebras by part~\ref{homogeneous basis for associated graded of weyl algebra}.
    \qedhere
  \end{enumerate}
\end{proof}


\begin{remark}
  The Weyl algebra is an example of a \defemph{skew polynomial ring}:
  If~$R$ is a~{\algebra{$\kf$}} and~$\delta$ is a derivation of~$R$ then one can endow the polynomial vector space~$A = R[t]$ uniquely with the structure of a~{\algebra{$\kf$}} -- different from the usual one unless~$\delta = 0$ -- such that
  \begin{itemize*}
    \item
      the inclusion from~$R$ to~$A$ given by~$r \mapsto r t^0$ is a homomorphism of~\algebras{$\kf$},
    \item
      $t^i$ is the~{\howmanyth{$i$}} power of~$t$ in~$A$, and
    \item
      the variable~$t$ interacts with the elements~$r$ of~$R$ via~$tr = rt + \delta(r)$.
  \end{itemize*}
  The resulting~{\algebra{$\kf$}} is a \defemph{skew polynomial algebra}\index{skew polyomial algebra} over~$R$ and denoted by~\gls*{skew polynomial algebra}.
  The multiplication of~$R[t;\delta]$ is built precisely so that the derivation~$[t,-]$ of~$R[t;\delta]$ acts on~$R t^0 \cong R$ by~$\delta$.
  More explicitely,
  \[
    [t, r t^0]
    =
    \delta(r) t^0
  \]
  for all~$r \in R$.
  The following two constructions are special cases of skew polynomial algebras.
  \begin{enumerate*}
    \item
      If~$R$ is any~\algebra{$\kf$} and~$\delta = 0$ then~$R[t; \delta]$ is the usual polynomial algebra~$R[t]$.
    \item
      If~$R$ is the polynomial algebra~$\kf[t]$ in a single variable~$t$ and~$\partial_t$ is the derivative with respect to the variable~$t$ than~$R[t;\partial_t]$ is the Weyl~algebra.
  \end{enumerate*}

%   Currently not needed and distracting.
%
%   Skew polynomial algebras can be further generalized:
%   If~$\sigma \colon R \to R$ is an algebra homomorphism then a~{\linear{$\kf$}} map~$\delta \colon R \to R$ is a~{\derivation{$\sigma$}}\index{$\sigma$-derivation}\index{derivation!$\sigma$-} if
%   \[
%     \delta(rs)
%     =
%     \delta(r) s + \sigma(r) \delta(s)
%   \]
%   for all~$r, s \in R$.
%   Then the polynomial vector space~$A = R[t]$ can be endowed uniquely with the structure of a~{\algebra{$\kf$}} such that
%   \begin{itemize}
%     \item
%       the inclusion~$R \to A$,~$r \mapsto r t^0$ is a homomorphism of~{\algebras{$\kf$}},
%     \item
%       $t^i$ is the~{\howmanyth{$i$}} power of~$t$ in~$A$ and
%     \item
%       the variable~$t$ interacts with the elements~$r \in R$ via~$t r = \sigma(r) t + \delta(r)$.
%   \end{itemize}
%   The resulting algebra~$A$ is an \defemph{Ore extension}\index{Ore extension} of~$R$ and is denoted by~\gls*{ore extension}.
\end{remark}


\begin{remark}[Weyl and Heisenberg]
  The Weyl~algebra~$A$ is connected to the {\threedimensional} Heisenberg~Lie~algebras~$\Hlie$ as follows.

  The Lie~algebra~$\Hlie$ has a basis~$p$,~$q$,~$c$ on which the Lie~bracket is given by~$[p,c], [q,c] = 0$ and~$[p,q] = c$.
  The element~$c$ is central in~$\glie$.
  The Weyl~algebra~$A$ results from the universal enveloping algebra~$\Univ(\Hlie)$ by~\enquote{setting~$c$ equal to~$1$}.
  More precisely, we have that
  \[
    \Univ(\Hlie) / \ideal{ \class{c} - 1 }
    \cong
    A
  \]
  with the elements~$\class{p}$ and~$\class{q}$ of~$\Univ(\Hlie)$ corresponding to the elements~$y$ and~$x$ of~$A$.
  To formally prove this we abbreviate~$\Univ(\Hlie)/(\class{c} - 1)$ as~$B$.
  
  Let~$\varphi$ be the unique linear map from~$\Hlie$ to~$A$ given by
  \[
    \varphi(p) = y \,,
    \quad
    \varphi(q) = x \,,
    \quad
    \varphi(c)  =1 \,.
  \]
  This maps is a homomorphism of Lie~algebras and thus induces a homomorphism of algebras~$\Phi$ from~$\Univ(\Hlie)$ to~$A$.
  This homomorphism~$\Phi'$ is given on the algebra generators~$\class{p}$,~$\class{q}$,~$\class{c}$ of~$\Univ(\Hlie)$ by
  \[
    \Phi'( \class{p} ) = y \,,
    \quad
    \Phi'( \class{q} ) = x \,,
    \quad
    \Phi'( \class{c} ) = 1 \,.
  \]
  It holds that
  \[
    \Phi'(\class{c} - 1)
    =
    \Phi'(\class{c}) - \Phi'(1)
    =
    1 - 1
    =
    0 \,,
  \]
  whence~$\Phi'$ descends to a well-defined algebra homomorphism~$\Phi$ from~$B$ to~$A$.
  The homomorphism~$\Phi$ is given on the remaining algebra generators~$\class{p}$ and~$\class{q}$ of~$B$ by
  \[
    \Phi(\class{p}) = y \,,
    \quad
    \Phi(\class{q}) = x \,.
  \]
  
  To construct the inverse homomorphism~$\Psi$ of~$\Phi$ we can start off with the unique algebra homomorphism~$\Psi'$ from~$\kf\gen{X,Y}$ to~$B$ which is given on the free variables~$X$ and~$Y$ by
  \[
    \Psi'(X) = \class{q} \,,,
    \quad
    \Psi'(Y) = \class{p} \,.
  \]
  Then
  \[
    \Psi'(YX)
    =
    \class{p} \, \class{q}
    =
    \class{q} \, \class{p} + \class{[p,q]}
    =
    \class{q} \, \class{p} + \class{c}
    =
    \class{q} \, \class{p} + 1
    =
    \Psi'(XY + 1)
  \]
  and therefore~$\Psi'(YX - XY - 1) = 0$.
  It follows that the homomorphism~$\Psi'$ factors uniquely through a homomorphism of algebras~$\Psi$ from~$A$ to~$B$ which is given on the algebra generators~$x$ and~$y$ of~$A$ by~$\Psi(x) = \class{q}$ and~$\Psi(y) = \class{p}$.
  
  The two homomorphisms~$\Phi$ are~$\Psi$ are mutually inverse on the algebra generators~$y$,~$x$ of~$A$ and~$\class{p}$,~$\class{q}$ of~$B$.
  This means that~$\Phi$ and~$\Psi$ are mutually inverse isomorphisms.
\end{remark}


\begin{remark}
  \Cref{representation theory trick to construct a basis} generalizes to other algebraic structures, for example groups.
  \begin{enumerate}
    \item
      If~$X$ is a set and~$F$ is the free group on~$X$ then every element of~$F$ can be uniquely written as a reduced word in the alphabet~$X^{\pm 1}$.
      The uniqueness of such a reduced expression can be shown by letting~$F$ act on the set of all reduced words.
    \item
      Let~$G_i$ with~$i$ in~$I$ be a collection of groups and let~$H$ be a group.
      For every index~$i$ in~$I$ let~$f_i$ be a homomorphism of groups from~$H$ to~$G_i$.
      Then elements of the resulting amalgamated product~$A = \bigast_{H,i \in I} G_i$ can be represented in certain a canonical form, the uniqueness of which can be shown by letting~$A$ act on the set of all possible canonical forms.
      We refer to \cite[\S 1.2]{trees} for more information on this example.
  \end{enumerate}
\end{remark}


% Bad example: Already graded
%
% \begin{example}[Quantum plane]
%   Let~$q \in \kf$ wit~$q \neq 0$.
%   The \emph{quantum plane} is the~{\algebra{$\kf$}}~$A \defined \kf\gen{X,Y}/(YX - qXY)$.%
%   \footnote{The usual polynomial ring~$\kf[x,y] \cong \kf\gen{X,Y}/(YX - XY)$ is the algebraic object corresponding to the plane~$\Aff^2 = k^2$ in the sense that~$\kf[x,y]$ is the algebra of (regular) functions on~$\Aff^2$.
%   The given algebra~$A$ should therefore correspond to some (non-existing) plane, the functions on which don’t commute.}
%   Let~$x, y \in A$ be the residue classes of~$X$ and~$Y$.
%   The~{\algebra{$\kf$}}~$A$ inherits from the standard grading of the free algebra~$\kf\gen{X,Y}$ a filtration given by
%   \[
%     A_{(p)}
%     =
%     \gen{
%       z_1 \dotsm z_q
%     \suchthat
%       0 \leq j \leq i,
%       z_1, \dotsc, z_q \in \{x, y\}
%     }_{\kf} \,.
%   \]
%   It can be shown as for the Weyl~algebra (actually easer than for the Weyl~algebra) for all~$i \geq 0$ the vector space~$A_{(p)}$ is spanned by the monomials~$x^n y^m$ with~$n + m \leq i$.
%   The quotient vector space~$\gr[p](A)$ is therefore spanned for every~$i \geq 0$ by the residue classes~$[x^n y^m]_p$ with~$n + m = i$.
%   The algebra~$\gr(A)$ is hence spanned by the collection of all such residue classes~$[x^n y^m]$ with~$n, m \geq 0$.
% \end{example}


\begin{warning}
  Let~$A$ be a filtered~\algebra{$\kf$}.
  There does not exist a \enquote{canonical} algebra homomorphism from~$A$ to~$\gr(A)$.
  There does not even have to exist any homomorphism of algebras from~$A$ to~$\gr(A)$.

  As an example we consider for~$A$ the Weyl algebra with the filtration from \cref{results about the weyl algerba}.
  The associated graded algebra~$\gr(A)$ is isomorphic to the polynomial algebra~$\kf[t,u]$, and it is therefore in particular commutative.
  The homomorphisms of algebras from~$A$ to~$\gr(A)$ correspond bijectively to pairs~$(x, y)$ consisting of elements of $\gr(A)$ which satisfy the commutator relation~$yx - xy - 1 = 0$.
  But no such pair exists because the algebra~$\gr(A)$ is commutative.
  There hence exist no homomorphism of algebras from~$A$ to~$\gr(A)$.
\end{warning}





